Engine/Tree: rename first_branch'

Semantics/Tree.v
@@ -158,7 +158,7 @@ Section Tree.
   Definition first_branch (t:tree) (str0: string) : option leaf :=
     tree_res t GroupMap.empty (init_input str0) forward.
 
-  Definition first_branch' (t:tree) (inp:input) : option leaf :=
+  Definition first_leaf (t:tree) (inp:input) : option leaf :=
     tree_res t GroupMap.empty inp forward.
 
   (** * All Tree Results *)
